wrote SortedListOrder

theories/certs/footer.v
@@ -1,11 +1,6 @@
-Definition sorted_order := Eval compute in sort <%O final_order.
-
-Definition reorderK := @pordK _ final_order sorted_order
-                      is_true_true is_true_true.
-
 Theorem isopres_final : isopres present_entry present_final.
 Proof.
-have wfc : wfpres_cert present_entry cert by vm_cast_no_check (eq_refl true).
+have wfc : wfpres_cert present_entry cert by vm_cast_no_check is_true_true.
 apply: (isopres_trans (@iso_final_pres _ present_entry cert wfc)).
 apply: pres_irrelevance.
   by rewrite (pgen_final_pres wfc).
@@ -14,15 +9,15 @@ Time Qed.
 
 Theorem final_ok : convergent (prelat present_final).
 Proof.
-apply: (rgen_convergent reorderK erefl).
+apply: (rgen_convergent (reorderK (l := final_order) is_true_true) erefl).
 apply: diamond.
   apply: (decreasing_wf (@lt_sizelexi_stable _ int) sizelexi_int_wf).
-  by native_cast_no_check (eq_refl true).
+  by native_cast_no_check is_true_true.
 apply: (spair_confluenceP (fuel := 20)).
 rewrite spair_confluence_dec_intE.
 (* Set NativeCompute Timing.
 Set NativeCompute Profiling.
 Time by native_compute.  *)
-by native_cast_no_check (eq_refl true).
+by native_cast_no_check is_true_true.
 (* Optimize Heap. *)
 Time Qed.
